pcuic/theories/PCUICElimination.v
@@ -738,6 +738,19 @@ Proof.
   eapply cumul_sprop_props in leq; auto. eauto. auto. apply wfΣ.
 Qed.
 
+Lemma leq_term_propositional_sorted_l {Σ Γ v v' u u'} :
+  wf_ext Σ ->
+  PCUICEquality.leq_term Σ (global_ext_constraints Σ) v v' ->
+  Σ;;; Γ |- v : tSort u ->
+  Σ;;; Γ |- v' : tSort u' -> is_propositional u -> 
+  leq_universe (global_ext_constraints Σ) u' u.
+Proof.
+  intros wfΣ leq hv hv' isp.
+  eapply orb_true_iff in isp as [isp | isp].
+  - eapply leq_term_prop_sorted_l; eauto.
+  - eapply leq_term_sprop_sorted_l; eauto.
+Qed.
+
 Lemma leq_term_sprop_sorted_r {Σ Γ v v' u u'} :
   wf_ext Σ ->
   PCUICEquality.leq_term Σ (global_ext_constraints Σ) v v' ->
