translations/times_bool_fun2.v
@@ -4,7 +4,7 @@ Unset Universe Checking.
 From MetaCoq.Translations Require Import translation_utils times_bool_fun MiniHoTT.
 Import MCMonadNotation.
 
-Unset Strict Unquote Universe Mode.
+Unset MetaCoq Strict Unquote Universe Mode.
 
 MetaCoq Run (TC <- ImplementExisting emptyTC "paths" ;;
                      TC <- ImplementExisting TC "idpath" ;;
